dafny 4 updates and various lemmas in DiameterOfBinaryTree.dfy

lib/seq.dfy
@@ -1,15 +1,15 @@
 
 module Seq {
-    predicate substring1<A>(sub: seq<A>, super: seq<A>) {
+    predicate substring1<A(==)>(sub: seq<A>, super: seq<A>) {
         exists k :: 0 <= k < |super| && sub <= super[k..]
     }
 
 
-    predicate isSubstringAlt<A(!new)>(sub: seq<A>, super: seq<A>) {
+    ghost predicate isSubstringAlt<A(!new)>(sub: seq<A>, super: seq<A>) {
         |sub| <= |super| && exists xs: seq<A> :: IsSuffix(xs, super) && sub <= xs
     }
 
-    predicate isSubstring<A>(sub: seq<A>, super: seq<A>) {
+    predicate isSubstring<A(==)>(sub: seq<A>, super: seq<A>) {
         |sub| <= |super| && exists k,j :: 0 <= k < j <= |super| && sub == super[k..j]
     }
 
@@ -18,29 +18,60 @@ module Seq {
         requires 0 <= s <= t <= j-k
         ensures xs[k..j][s..t] == xs[(k+s)..(k+s+(t-s))]
     {
-        // if k == 0 && j == 0 {
-        //     assert xs[k..j] == [];
-        //     assert xs[k..j][s..t] == [];
-        // }else if k == 0 && j == |xs| {
-        //     assert xs[k..j] == xs;
-        //     assert xs[k..j][s..t] == xs[(k+s)..(k+s+t-s)];
-        // }else if k == |xs| && j == |xs| {
-        //     assert xs[k..j] == [];
-        //     assert xs[k..j][s..t] == xs[(k+s)..(k+s+t-s)];
-        // }else 
-        if 0 <= k <= j <= |xs| {
             if j-k == 0 {
-
             }else if t-s == 0 {
-
             }else if t-s > 0 {
                 SliceOfSliceIsSlice(xs, k, j, s,t-1);
                 assert xs[k..j][s..t] == xs[k..j][s..(t-1)]+[xs[k..j][t-1]];
             }
-        }else{
-            assert false;
-        }
     }
+
+    lemma notInNotEqual<A>(xs: seq<A>, elem: A)
+        requires elem !in xs
+        ensures forall k :: 0 <= k < |xs| ==> xs[k] != elem
+    {
+
+    }
+
+    predicate injectiveSeq<A(==)>(s: seq<A>) {
+        forall x,y :: x != y && 0 <= x <= y < |s| ==> s[x] != s[y]
+    }
+
+    lemma injectiveSeqs<A>(xs: seq<A>, ys: seq<A>)
+        requires injectiveSeq(xs)
+        requires injectiveSeq(ys)
+        requires forall x :: x in xs ==> x !in ys 
+        requires forall y :: y in ys ==> y !in xs 
+        ensures injectiveSeq(xs+ys)
+    {
+        var len := |xs + ys|;
+        forall x,y | x != y && 0 <= x <= y < |xs+ys| 
+            ensures (xs+ys)[x] != (xs+ys)[y] 
+        {
+            if 0 <= x < |xs| && 0 <= y < |xs| {
+                assert (xs+ys)[x] != (xs+ys)[y];
+            }else if |xs| <= x < |xs+ys| && |xs| <= y < |xs+ys| {
+                assert (xs+ys)[x] != (xs+ys)[y];
+
+            }else if 0 <= x < |xs| && |xs| <= y < |xs+ys| {
+                notInNotEqual(ys, xs[x]);
+                assert (xs+ys)[x] != (xs+ys)[y];
+            }
+        }
+
+    }
+
+    // if k == 0 && j == 0 {
+    //     assert xs[k..j] == [];
+    //     assert xs[k..j][s..t] == [];
+    // }else if k == 0 && j == |xs| {
+    //     assert xs[k..j] == xs;
+    //     assert xs[k..j][s..t] == xs[(k+s)..(k+s+t-s)];
+    // }else if k == |xs| && j == |xs| {
+    //     assert xs[k..j] == [];
+    //     assert xs[k..j][s..t] == xs[(k+s)..(k+s+t-s)];
+    // }else 
+    // if 0 <= k <= j <= |xs| {
 
     lemma AllSubstringsAreSubstrings<A>(subsub: seq<A>, sub: seq<A>, super: seq<A>)
         requires isSubstring(sub, super)
@@ -78,19 +109,147 @@ module Seq {
         } else if t <= j {
 
         }
-        var z,q :| 0 <= z <= q <= |super| && super[z..q] == super[k..j][s..t];
+        // var z,q :| 0 <= z <= q <= |super| && super[z..q] == super[k..j][s..t];
     }
 
 
-    predicate IsSuffix<T>(xs: seq<T>, ys: seq<T>) {
+    predicate IsSuffix<T(==)>(xs: seq<T>, ys: seq<T>) {
         |xs| <= |ys| && xs == ys[|ys| - |xs|..]
     }
 
-    predicate IsSuffix2<T>(xs: seq<T>, ys: seq<T>) {
+    predicate IsSuffix2<T(==)>(xs: seq<T>, ys: seq<T>) {
         |xs| <= |ys| && exists K :: 0 <= K <= |ys|-|xs| && ys == ys[0..K] + xs + ys[(K+|xs|)..]
     }
 
-    method Test() {
+    function reverse<A>(x: seq<A>): seq<A> 
+
+    {
+        if x == [] then [] else reverse(x[1..])+[x[0]]
+    }
+
+    lemma {:induction false} reversePreservesMultiset<A>(xs: seq<A>) 
+        ensures multiset(xs) == multiset(reverse(xs))
+    {
+        if xs == [] {
+
+        }else {
+            var x := xs[0];
+            assert xs == [x] + xs[1..];
+            assert multiset(xs) == multiset([x]) + multiset(xs[1..]);
+            assert reverse(xs) == reverse(xs[1..])+[x];
+            reversePreservesMultiset(xs[1..]);
+            assert multiset(xs[1..]) == multiset(reverse(xs[1..]));
+        }
+    }
+
+    lemma  reversePreservesLength<A>(xs: seq<A>)
+        ensures |xs| == |reverse(xs)|
+    {
+
+    }
+
+    lemma  lastReverseIsFirst<A>(xs: seq<A>)
+        requires |xs| > 0
+        ensures xs[0] == reverse(xs)[|reverse(xs)|-1]
+    {
+        reversePreservesLength(xs);
+        assert |xs| == |reverse(xs)|;
+    }
+
+    lemma firstReverseIsLast<A>(xs: seq<A>)
+        requires |xs| > 0
+        ensures reverse(xs)[0] == xs[|xs|-1]
+    {
+
+    }
+
+    lemma ReverseConcat<T>(xs: seq<T>, ys: seq<T>)
+        ensures reverse(xs + ys) == reverse(ys) + reverse(xs)
+    {
+        // reveal Reverse();
+        if |xs| == 0 {
+        assert xs + ys == ys;
+        } else {
+        assert xs + ys == [xs[0]] + (xs[1..] + ys);
+        }
+    }
+
+
+    lemma reverseRest<A>(xs: seq<A>)
+        requires |xs| > 0
+        ensures reverse(xs) == [xs[ |xs| -1 ] ] + reverse(xs[0..|xs|-1])
+    {
+        firstReverseIsLast(xs);
+        assert xs == xs[0..|xs|-1] + [xs[|xs|-1]];
+        assert reverse(xs)[0] == xs[ |xs| -1];
+        assert reverse(xs) == [xs[ |xs| -1]] + reverse(xs)[1..];
+        calc {
+            reverse(xs);
+            reverse(xs[0..|xs|-1] + [xs[|xs|-1]]);
+            == {ReverseConcat(xs[0..|xs|-1], [xs[ |xs|-1 ]]);}
+            reverse([xs[ |xs|-1 ]]) + reverse(xs[0..|xs|-1]);
+
+        }
+
+    }
+
+    lemma ReverseIndexAll<T>(xs: seq<T>)
+        ensures |reverse(xs)| == |xs|
+        ensures forall i :: 0 <= i < |xs| ==> reverse(xs)[i] == xs[|xs| - i - 1]
+    {
+    // reveal Reverse();
+    }
+
+    lemma ReverseIndex<T>(xs: seq<T>, i: int)
+        requires 0 <= i < |xs|
+        ensures |reverse(xs)| == |xs|
+        ensures reverse(xs)[i] == xs[|xs| - i - 1]
+    {
+        ReverseIndexAll(xs);
+        assert forall i :: 0 <= i < |xs| ==> reverse(xs)[i] == xs[|xs| - i - 1];
+    }
+
+    lemma ReverseSingle<A>(xs: seq<A>) 
+        requires |xs| == 1
+        ensures reverse(xs) == xs
+    {
+
+    }
+
+    lemma SeqEq<T>(xs: seq<T>, ys: seq<T>)
+        requires |xs| == |ys|
+        requires forall i :: 0 <= i < |xs| ==> xs[i] == ys[i]
+        ensures xs == ys
+    {
+    }
+
+    lemma reverseReverseIdempotent<A>(xs: seq<A>) 
+        ensures reverse(reverse(xs)) == xs
+    {
+        if xs == [] {
+
+        }else{
+            calc {
+                reverse(reverse(xs));
+                reverse(reverse([xs[0]] + xs[1..]));
+                == {ReverseConcat([xs[0]] , xs[1..]);}
+                reverse(reverse(xs[1..]) + reverse([xs[0]]));
+                == {ReverseSingle([xs[0]]);}
+                reverse(reverse(xs[1..]) + [xs[0]]);
+                == {ReverseConcat(reverse(xs[1..]), [xs[0]]);}
+                reverse([xs[0]]) + reverse(reverse(xs[1..]));
+                [xs[0]] + reverse(reverse(xs[1..]));
+                == {reverseReverseIdempotent(xs[1..]);}
+                xs;
+            }
+        }
+        /* Alternatively */
+        // ReverseIndexAll(reverse(xs));
+        // ReverseIndexAll(xs);
+        // SeqEq(reverse(reverse(xs)), xs);
+    }
+
+    method SeqTest() {
         var t1 := [4,5,6,1,2,3];
         // assert t1 == [4,5,6]+[1,2,3];
         var s1 := [1,2,3];
