leetcode/DiameterOfBinaryTree.dfy
@@ -1,0 +1,615 @@
+//https://leetcode.com/problems/diameter-of-binary-tree/description/
+
+/*
+function diameter(node: TreeNode | null): [number, number] {
+  if(node == null) {
+    return [-1,-1];
+  }
+  if(node.left == null && node.right == null) {
+    return [0, 0];
+  }
+  let leftDiameter = diameter(node.left);
+  let rightDiameter = diameter(node.right);
+  let height = Math.max(leftDiameter[0],rightDiameter[0]) + 1;
+  let dim = leftDiameter[0]+rightDiameter[0]+2;
+  let maxDiameter = Math.max(leftDiameter[1], rightDiameter[1], dim);
+  return [height, maxDiameter];
+}
+
+function diameterOfBinaryTree(root: TreeNode | null): number {
+  return diameter(root)[1];
+};
+*/
+// include "../lib/seq.dfy"
+include "../lib/binaryTree.dfy"
+import opened BinaryTree
+// import opened Seq
+function reverse<A(==)>(x: seq<A>): seq<A> 
+
+{
+    if x == [] then [] else reverse(x[1..])+[x[0]]
+}
+
+lemma notInNotEqual<A(==)>(xs: seq<A>, elem: A)
+    requires elem !in xs
+    ensures forall k :: 0 <= k < |xs| ==> xs[k] != elem
+{
+
+}
+
+predicate injectiveSeq<A(==)>(s: seq<A>) {
+    forall x,y :: x != y && 0 <= x <= y < |s| ==> s[x] != s[y]
+}
+
+lemma injectiveSeqs<A>(xs: seq<A>, ys: seq<A>)
+    requires injectiveSeq(xs)
+    requires injectiveSeq(ys)
+    requires forall x :: x in xs ==> x !in ys 
+    requires forall y :: y in ys ==> y !in xs 
+    ensures injectiveSeq(xs+ys)
+{
+    var len := |xs + ys|;
+    forall x,y | x != y && 0 <= x <= y < |xs+ys| 
+        ensures (xs+ys)[x] != (xs+ys)[y] 
+    {
+        if 0 <= x < |xs| && 0 <= y < |xs| {
+            assert (xs+ys)[x] != (xs+ys)[y];
+        }else if |xs| <= x < |xs+ys| && |xs| <= y < |xs+ys| {
+            assert (xs+ys)[x] != (xs+ys)[y];
+
+        }else if 0 <= x < |xs| && |xs| <= y < |xs+ys| {
+            notInNotEqual(ys, xs[x]);
+            assert (xs+ys)[x] != (xs+ys)[y];
+        }
+    }
+
+}
+
+function max(left: int, right: int): int {
+    if left > right then left else right
+}
+
+function TreeSet(root: Tree): set<Tree> {
+    match root {
+        case Nil => {}
+        case Node(val, left, right) => {root}+TreeSet(left)+TreeSet(right)
+    }
+}
+
+function TreeHeight(root: Tree): int 
+    ensures TreeHeight(root) >= -1
+{
+    if root == Nil then -1 else if root.left == Nil && root.right == Nil then 0 else max(TreeHeight(root.left), TreeHeight(root.right)) + 1
+}
+
+predicate isPath(paths: seq<Tree>) {
+    if |paths| == 0 then false else if |paths| == 1 then match paths[0] {
+        case Nil => false
+        case Node(val, left, right) => true
+    } else match paths[0] {
+        case Nil => false
+        case Node(val, left, right) => (left == paths[1] || right == paths[1] || (paths[1] != Nil && (paths[0] == paths[1].left || paths[0] == paths[1].right))) && isPath(paths[1..])
+    }
+}
+
+predicate isValidTreePath(path: seq<Tree>, start: Tree, end: Tree) {
+    isTreePath(path, start, end) && exists root: Tree :: root != Nil && root in path && (forall node: Tree :: (node in path) ==> node in TreeSet(root))
+}
+
+predicate isTreePath(path: seq<Tree>, start: Tree, end: Tree) {
+    if |path| == 0 then false else if |path| == 1 then start != Nil && start == end && path[0] == start else match path[0] {
+        case Nil => false
+        case Node(val, left, right) => path[0] == start && (left == path[1] || right == path[1] || (path[1] != Nil && (path[0] == path[1].left || path[0] == path[1].right))) && isTreePath(path[1..], path[1], end)
+    }
+}
+
+predicate isDescTreePath(path: seq<Tree>, start: Tree, end: Tree) {
+    if |path| == 0 then false else if |path| == 1 then match path[0] {
+            case Nil => false
+            case Node(val, left, right) => path[0] == start && end == start
+    } else match path[0] {
+        case Nil => false
+        case Node(val, left, right) => end != Nil && path[|path|-1] == end && path[0] == start && path[1] != Nil && ((left == path[1] && isDescTreePath(path[1..],left, end)) || (right == path[1] && isDescTreePath(path[1..], right, end)))
+    }
+}
+
+predicate isAscTreePath(paths: seq<Tree>, start: Tree, end: Tree) {
+    if |paths| == 0 then false else if |paths| == 1 then match paths[0] {
+        case Nil => false
+        case Node(val, left, right) => start == paths[0] && end == start
+    } else match paths[0] {
+        case Nil => false
+        case Node(val, left, right) => end != Nil && paths[|paths|-1] == end && start == paths[0] && paths[1] != Nil  && ((paths[0] == paths[1].left && isAscTreePath(paths[1..], paths[1], end)) || (paths[0] == paths[1].right && isAscTreePath(paths[1..], paths[1], end)))
+    }
+}
+
+
+predicate isAscPath(paths: seq<Tree>, root: Tree) {
+    if |paths| == 0 then false else if |paths| == 1 then match paths[0] {
+        case Nil => false
+        case Node(val, left, right) => root == paths[0]
+    } else match paths[0] {
+        case Nil => false
+        case Node(val, left, right) => root == paths[0] && paths[1] != Nil && isAscPath(paths[1..], paths[1]) && (paths[0] == paths[1].left  || paths[0] == paths[1].right)
+    }
+}
+
+predicate isDescPath(paths: seq<Tree>, root: Tree) {
+    if |paths| == 0 then false else if |paths| == 1 then match paths[0] {
+        case Nil => false
+        case Node(val, left, right) => paths[0] == root
+    } else match paths[0] {
+        case Nil => false
+        case Node(val, left, right) => paths[0] == root && ((left == paths[1] && isDescPath(paths[1..], left)) || (right == paths[1] && isDescPath(paths[1..], right)))
+    }
+}
+
+
+
+lemma TreeSetChildInTreeSet(root: Tree, child: Tree) 
+    requires root != Nil
+    requires child != Nil && child in TreeSet(root)
+    ensures TreeSet(child) <= TreeSet(root)
+{}
+
+lemma parentNotInTreeSet(parent: Tree, root: Tree)
+    requires parent != Nil && parent != root && (parent.left == root || parent.right == root)
+    ensures parent !in TreeSet(root)
+{
+    if root == Nil {} else {
+        assert TreeSet(root) == {root}+TreeSet(root.left)+TreeSet(root.right);
+        parentNotInTreeSet(root, root.left);
+        parentNotInTreeSet(root, root.right);
+        if parent in TreeSet(root.left) {
+            TreeSetChildInTreeSet(root.left, parent);
+        }else if parent in TreeSet(root.right) {
+            TreeSetChildInTreeSet(root.right, parent);
+        }
+    }
+}
+// assert root !in TreeSet(root.left);
+// assert root !in TreeSet(root.right);
+// assert parent !in {root};
+// assert parent in TreeSet(root.left)+TreeSet(root.right);
+
+lemma {:verify false} isPathKinds(paths: seq<Tree>, root: Tree)
+    requires validPath(paths, root)
+    ensures isDescPath(paths, root) || isAscPath(paths, root) || exists k: nat :: k < |paths| && paths == paths[0..k] + paths[k..] && isAscPath(paths[0..k], root) && isDescPath(paths[k..], root)
+{
+    assert |paths| > 0;
+    if |paths| == 1 {
+
+    } else if paths[0] == root {
+        if isDescPath(paths, root) {
+
+        }else{
+            assert !((root.left == paths[1] && isDescPath(paths[1..], root.left)) || (root.right == paths[1] && isDescPath(paths[1..], root.right)));
+            assert !(root.left == paths[1] && isDescPath(paths[1..], root.left)) && !(root.right == paths[1] && isDescPath(paths[1..], root.right));
+            assert (root.left != paths[1] || !isDescPath(paths[1..], root.left)) && (root.right != paths[1] || !isDescPath(paths[1..], root.right));
+            if root.left != paths[1] || !isDescPath(paths[1..], root.left) {
+                if root.left != paths[1] && isDescPath(paths[1..], root.left) {
+                    assert false;
+                } else if root.left == paths[1] && !isDescPath(paths[1..], root.left) {
+                    
+                }
+
+            } else if root.right != paths[1] || !isDescPath(paths[1..], root.right) {
+
+                if root.right != paths[1] && isDescPath(paths[1..], root.right) {
+
+                } else if root.right == paths[1] && !isDescPath(paths[1..], root.right) {
+
+                }
+            }
+            assert false;
+        }
+    } else if paths[|paths|-1] == root {
+
+    }else{
+
+    }
+}
+
+
+method TestPath() {
+    var rootleaf := Node(4, Nil, Nil);
+    var leaf := Node(3, Nil, Nil);
+    var child := Node(2, Nil, leaf);
+    var root := Node(1, child, rootleaf);
+    assert isPath([leaf, child, root]);
+    // assert isPath([leaf, child, root, rootleaf]);
+    assert !isTreePath([root, rootleaf], leaf, rootleaf);
+    assert isTreePath([leaf, child, root], leaf, root);
+    assert isTreePath([root, rootleaf], root, rootleaf);
+    assert isTreePath([leaf, child, root, rootleaf], leaf, rootleaf);
+    assert isPath([root, child, leaf]);
+    assert isDescPath([root, child, leaf], root);
+    assert isDescTreePath([root, child, leaf], root, leaf);
+    assert !isDescTreePath([root], root, leaf);
+    assert isDescTreePath([root, rootleaf],root, rootleaf);
+    assert isPath([root, child]);
+    assert isPath([child, leaf]);
+    assert isPath([leaf, child]);
+    // assert isTreePath([leaf], leaf, leaf);
+    // assert isTreePath([child], child, child);
+    // assert isTreePath([leaf,child], leaf, child);
+    assert isTreePath([leaf,child,root], leaf, root);
+    assert isTreePath([root,child,leaf], root, leaf);
+}
+
+predicate validPath(path: seq<Tree>, root: Tree) {
+    isPath(path) && forall node :: node in path ==> node in TreeSet(root) && root in path
+}
+
+lemma {:verify false} AscPathIsDescPath(path: seq<Tree>, start: Tree, end: Tree)
+    requires start != Nil
+    requires end != Nil
+    requires |path| >= 1
+    requires isAscTreePath(path, start, end)
+    ensures isDescTreePath(reverse(path), end, start)
+{
+    assert path[0] == start;
+    assert path[ |path| - 1] == end;
+}
+
+lemma {:verify false} TreeHeightToDescPath(root: Tree, h: int)
+    requires root != Nil
+    requires h == TreeHeight(root)
+    ensures exists path: seq<Tree> :: isDescPath(path, root)
+{
+    if h == 0 {
+        assert isDescPath([root], root);
+    }else if h > 0 {
+
+    }
+}
+
+lemma  TreeHeightLeaf(root: Tree)
+    requires root != Nil
+    requires TreeHeight(root) == 0
+    ensures root.left == Nil && root.right == Nil
+{}
+
+lemma TreeHeightToDescTreePath(root: Tree, h: int) 
+    requires root != Nil
+    requires h == TreeHeight(root)
+    ensures exists end: Tree, path: seq<Tree> :: (end != Nil && end.left == Nil && end.right == Nil)  && isDescTreePath(path, root, end) && |path| == h+1
+{
+    if h == 0 {
+        assert isDescTreePath([root], root, root);
+    }else if h >= 1 {
+        if root.left != Nil && TreeHeight(root.left) == h-1 {
+            TreeHeightToDescTreePath(root.left, h-1);
+            var end: Tree, path: seq<Tree> :| end != Nil && end.left == Nil && end.right == Nil && isDescTreePath(path, root.left, end) && |path| == h;
+            assert end != Nil && isDescTreePath([root]+path, root, end) && |[root]+path| == h+1;
+        } else if root.right != Nil && TreeHeight(root.right) == h-1 {
+            TreeHeightToDescTreePath(root.right, h-1);
+            var end: Tree, path: seq<Tree> :| end != Nil && end.left == Nil && end.right == Nil && isDescTreePath(path, root.right, end) && |path| == h;
+            assert end != Nil && isDescTreePath([root]+path, root, end) && |[root]+path| == h+1;
+        }
+    }
+}
+
+lemma DescTreePathNoChildren(path: seq<Tree>, root: Tree, end: Tree)
+    requires root != Nil
+    requires end != Nil
+    requires |path| > 1
+    requires isDescTreePath(path, root, end)
+    ensures forall x :: x in path[1..] ==> x in TreeSet(root) - {root} 
+{
+    if |path| == 2 {
+    }else{
+        if root.left != Nil && isDescTreePath(path[1..], root.left, end) {
+            parentNotInTreeSet(root,root.left);
+            forall x | x in path[1..] 
+                ensures x in TreeSet(root) - {root}
+            {
+                assert path[1..] == [path[1]]+path[2..];
+            }
+        }else if root.right != Nil && isDescTreePath(path[1..], root.right, end) {
+            parentNotInTreeSet(root,root.right);
+            forall x | x in path[1..] 
+                ensures x in TreeSet(root) - {root}
+            {
+                assert path[1..] == [path[1]] + path[2..];
+            } 
+        }
+    }
+}
+// assert path[2] != Nil;
+// assert root.left in TreeSet(root);
+// assert root !in TreeSet(root.left);
+// assert root.left in TreeSet(root) - {root};
+// DescTreePathNoChildren(path[2..], root.left, end); //required if induction false
+
+lemma DescTreePathInjective(path: seq<Tree>, root: Tree, end: Tree)
+    requires root != Nil
+    requires end != Nil
+    requires isDescTreePath(path, root, end)
+    ensures injectiveSeq(path)
+{
+    if |path| == 1 {
+
+    }else{
+        assert path[1] == root.left || path[1] == root.right;
+        assert root != root.left && root != root.right;
+        assert path == [root]+path[1..];
+        DescTreePathInjective(path[1..],path[1], end);
+        DescTreePathNoChildren(path, root, end);
+        // assert forall x :: x in path[1..] ==> x != root;
+        forall x,y | x != y && 0 <= x <= y < |path| 
+            ensures path[x] != path[y]; 
+        {
+            if x == 0 {
+                assert path[x] == root;
+                assert path[y] in path[1..];
+                assert path[y] != root;
+            }else{
+                assert path[x] != path[y];
+            }
+        }
+    }
+}
+
+lemma DescTreePathToPath(path: seq<Tree>, root: Tree, end: Tree)
+    requires root != Nil
+    requires end != Nil
+    requires isDescTreePath(path, root, end)
+    ensures isTreePath(path, root, end)
+{
+    assert path[0] == root;
+    assert path[|path|-1] == end;
+    if |path| == 1 {
+        assert path == [root];
+        assert isDescTreePath([root], root, end);
+        assert root == end;
+        assert isTreePath([root], root, end);
+    }
+}
+
+lemma DescTreePathSets(path: seq<Tree>, root: Tree, end: Tree)
+    requires root != Nil
+    requires end != Nil
+    requires isDescTreePath(path, root, end)
+    ensures forall node :: node in path ==> node in TreeSet(root)
+{}
+
+lemma AscTreePathNotNil(path: seq<Tree>, start: Tree, end: Tree)
+    requires start != Nil
+    requires end != Nil
+    requires |path| >= 1
+    requires isAscTreePath(path, start, end)
+    ensures forall node :: node in path ==> node != Nil
+{
+    if |path| == 1 {
+    }else if |path| > 1 {
+        assert path == [path[0]]+path[1..];
+        AscTreePathNotNil(path[1..], path[1], end);
+    }
+}
+
+lemma AscTreePathSlices(path: seq<Tree>, start: Tree, end: Tree)
+    requires start != Nil
+    requires end != Nil
+    requires isAscTreePath(path, start, end)
+    ensures forall k :: 0 <= k < |path| ==> isAscTreePath(path[k..], path[k], end);
+{
+
+}
+
+lemma {:verify false} AscTreePathSlicesBack(path: seq<Tree>, start: Tree, end: Tree)
+    requires start != Nil
+    requires end != Nil
+    requires isAscTreePath(path, start, end)
+    ensures forall k :: 0 < k < |path| ==> isAscTreePath(path[..k], start, path[k-1]);
+{
+    AscTreePathNotNil(path, start, end);
+    forall k | 0 < k < |path| 
+        ensures isAscTreePath(path[..k], start, path[k-1])
+    {
+        if k == 1 {
+
+        }else if k > 1{
+            var test := path[..k];
+            assert test[|test|-1] == path[k-1];
+            assert path[k-1] in path;
+            assert path[k-1] != Nil;
+            assert path[k-2] in path;
+            assert path[k-2] != Nil;
+            assert test[0] == start;
+            assert k-2 >= 0;
+            AscTreePathSlicesBack(path[..(k-1)], start, path[k-2]);
+        }
+    }
+}
+
+lemma {:verify false} {:induction false} AscTreePathSets(path: seq<Tree>, start: Tree, end: Tree)
+    requires start != Nil
+    requires end != Nil
+    requires isAscTreePath(path, start, end)
+    ensures forall node :: node in path ==> node in TreeSet(end)
+{
+    AscTreePathNotNil(path, start, end);
+    if |path| == 1 {
+
+    }else if |path| > 1 {
+        assert path[|path|-1] == end;
+        assert |path|-2 >= 0;
+        assert path[|path|-2] in path;
+        assert path[|path|-2] != Nil;
+        // assert isAscPath(paths[|])
+        assert path == path[0..|path|-2]+path[|path|-2..];
+        calc {
+            path[|path|-2..];
+            [path[|path|-2]]+path[|path|-1..];
+            [path[|path|-2]]+[path[ |path|-1]]+path[ |path|..];
+            [path[|path|-2]]+[path[ |path|-1]]+[];
+            [path[|path|-2] , path[ |path|-1]];
+        }
+        // assert path == path[0..|path|-2]+[path[|path|-2], path[|path|-1]];
+        AscTreePathSlices(path, start, end);
+        assert isAscTreePath(path[|path|-2..], path[|path|-2], end);
+        assert path[|path|-2..][1] == end;
+        // assert |path[|path|-2..]| == 2;
+        assert path[|path|-2] == end.right || path[|path|-2] == end.left;
+        assert isAscTreePath(path[..|path|-1], start, path[|path|-2]);
+    }
+}
+
+
+
+
+lemma {:induction false} ValidDescTreePathToPath(path: seq<Tree>, root: Tree, end: Tree)
+    requires root != Nil
+    requires end != Nil
+    requires isDescTreePath(path, root, end)
+    ensures isValidTreePath(path, root, end)
+{
+    if |path| == 1 {
+        assert path == [root];
+        assert isDescTreePath([root], root, end);
+        assert root in TreeSet(root);
+        assert root == end;
+        assert isTreePath([root], root, end);
+    }else if |path| > 1 {
+        assert path[0] == root;
+        assert root in path;
+        assert path[1] != Nil;
+        if path[1] == root.left {
+            ValidDescTreePathToPath(path[1..], root.left, end);
+            // TreeSetChildInTreeSet(root, root.left);
+            // assert isValidTreePath(path[1..], root.left, end);
+            DescTreePathSets(path[1..], root.left, end);
+            
+        } else if path[1] == root.right {
+            ValidDescTreePathToPath(path[1..], root.right, end);
+            // TreeSetChildInTreeSet(root, root.right);
+            DescTreePathSets(path[1..], root.right, end);
+
+        }
+    }
+}
+
+lemma DescPathToPath(path: seq<Tree>, root: Tree)
+    requires root != Nil
+    requires isDescPath(path, root)
+    ensures validPath(path, root)
+{
+    if |path| == 1 {
+        assert path == [root];
+        var ts := TreeSet(root);
+        assert forall x :: x in path ==> x in ts;
+        assert validPath([root], root);
+    }else if |path| > 1 {
+        assert path == [root]+path[1..];
+        assert path[1] != Nil;
+    }
+}
+
+lemma {:verify }  TreeHeightToTreePath(root: Tree, h: int)
+    requires root != Nil
+    requires h == TreeHeight(root)
+    ensures exists path: seq<Tree>, end: Tree :: isTreePath(path, root, end)// && |path| == h - 1
+{
+    TreeHeightToDescTreePath(root, h);
+    var end: Tree, path: seq<Tree> :| end != Nil && isDescTreePath(path, root, end);
+    DescTreePathToPath(path, root, end);
+}
+
+lemma Situation(path: seq<Tree>, root: Tree)
+    requires root != Nil
+    requires isDescPath(path, root.left)
+    ensures isDescPath([root]+path, root)
+    ensures isPath([root]+path)
+    ensures exists apath: seq<Tree> :: isPath(apath) && validPath(apath, root)
+{
+    DescPathToPath(path, root.left);
+    assert isPath(path);
+    var test := [root]+path;
+    assert isPath([root]+ path);
+}
+
+lemma SituationR(path: seq<Tree>, root: Tree)
+    requires root != Nil
+    requires isDescPath(path, root.right)
+    ensures isDescPath([root]+path, root)
+    ensures isPath([root]+path)
+    ensures exists apath: seq<Tree> :: isPath(apath) && validPath(apath, root)
+{
+    DescPathToPath(path, root.right);
+    assert isPath(path);
+    var test := [root]+path;
+    assert isPath([root]+ path);
+}
+
+lemma {:verify false} {:induction false} TreeHeightToPath(root: Tree, h: int)
+    requires root != Nil
+    requires h == TreeHeight(root)
+    ensures exists path: seq<Tree> :: validPath(path, root)// && |path| == h - 1
+{
+    if root.left == Nil && root.right == Nil {
+        assert h >= 0;
+        assert validPath([root], root);
+        assert TreeHeight(root) == 0;
+        assert exists path: seq<Tree> :: validPath(path, root);
+    }else if h > 0 {
+        assert h == max(TreeHeight(root.left), TreeHeight(root.right)) + 1;
+
+        assert h - 1 >= 0;
+        if TreeHeight(root.left) > TreeHeight(root.right) && TreeHeight(root.left) == h - 1 {
+            assert root.left != Nil;
+            TreeHeightToDescPath(root.left, h-1);
+            // var leftpath:seq<Tree> :| isValidPath(leftpath, root.left); 
+            var leftpath:seq<Tree> :| isDescPath(leftpath, root.left); 
+            Situation(leftpath, root);
+            TreeHeightToPath(root.left, h-1);
+            // var leftvalidpath: seq<Tree> :| validPath(leftvalidpath, root) && |leftvalidpath| == h - 2;
+            DescPathToPath(leftpath, root.left);
+            assert isPath(leftpath);
+            assert isPath([root]+leftpath);
+            assert validPath([root]+leftpath, root);
+            // assert |leftpath| == h-2;
+            // assert |[root]+leftpath| == h-1;
+            assert exists path: seq<Tree> :: validPath(path, root);
+        } else if TreeHeight(root.left) <= TreeHeight(root.right) && TreeHeight(root.right) == h - 1 {
+            assert root.right != Nil;
+            TreeHeightToDescPath(root.right, h-1);
+            var rightpath:seq<Tree> :| isDescPath(rightpath, root.right); 
+            SituationR(rightpath, root);
+            TreeHeightToPath(root.right, h-1);
+            DescPathToPath(rightpath, root.right);
+            assert validPath([root]+rightpath, root);
+            assert isPath(rightpath);
+            assert exists path: seq<Tree> :: validPath(path, root);
+        } else{
+            assert false;
+        }
+    }
+}
+
+method {:verify false} diameter(root: Tree) returns (heightDim: (int, int))
+    ensures heightDim.0 == TreeHeight(root)
+    ensures root != Nil ==> exists path: seq<Tree> :: isPath(path) && |path| - 1 == heightDim.1 && forall node :: node in path ==> node in TreeSet(root)
+{
+    if root == Nil {
+        return (-1, -1);
+    }
+    if root.left == Nil && root.right == Nil {
+        ghost var path := [root];
+        // assert isPath(path) && |path| - 1 == 0;
+        return (0,0);
+    }
+    var leftDiameter := diameter(root.left);
+    var rightDiameter := diameter(root.right);
+    var height := max(leftDiameter.0, rightDiameter.0) + 1;
+    var dim := leftDiameter.0 + rightDiameter.0 + 2;
+    var maxDiameter := max(leftDiameter.1, max(rightDiameter.1, dim));
+    return (height, maxDiameter);
+}
+
+method diameterOfBinaryTree(root: Tree) returns (maxDiameter: int)
+
+{
+    var result := diameter(root);
+    maxDiameter := result.1;
+}
